[minor] Change syscall model.
System calls are now performed in two steps, as suggested by
Benjamin. As expected, some of the proofs got simpler. Should be able to
call handler on system calls soon.

cfi/abstract.v
@@ -51,7 +51,7 @@ Open Scope word_scope.
 Local Notation word := (word t).
 Local Notation "x .+1" := (add_word x (Z_to_word 1)).
 
-Definition state := 
+Definition state :=
   (imemory * dmemory * registers * word (* pc *) * bool (*jump check*))%type.
 
 Record syscall := Syscall {
@@ -93,7 +93,7 @@ Inductive step : state -> state -> Prop :=
              forall (FETCH : get imem pc = Some i),
              forall (INST : decode_instr i = Some (Load _ r1 r2)),
              forall (R1W : get reg r1 = Some w1),
-             forall (MEM1 : get imem w1 = Some w2 \/ get dmem w1 = Some w2), 
+             forall (MEM1 : get imem w1 = Some w2 \/ get dmem w1 = Some w2),
              forall (UPD : upd reg r2 w2 = Some reg'),
              step (imem,dmem,reg,pc,true) (imem,dmem,reg',pc.+1,true)
 | step_store : forall imem dmem dmem' reg pc i r1 r2 w1 w2,
@@ -106,33 +106,29 @@ Inductive step : state -> state -> Prop :=
 | step_jump : forall imem dmem reg pc i r w b,
              forall (FETCH : get imem pc = Some i),
              forall (INST : decode_instr i = Some (Jump _ r)),
-             forall (RW : get reg r = Some w), 
-             forall (VALID : valid_jmp pc w = b), 
+             forall (RW : get reg r = Some w),
+             forall (VALID : valid_jmp pc w = b),
              step (imem,dmem,reg,pc,true) (imem,dmem,reg,w,b)
 | step_bnz : forall imem dmem reg pc i r n w,
              forall (FETCH : get imem pc = Some i),
              forall (INST : decode_instr i = Some (Bnz _ r n)),
              forall (RW : get reg r = Some w),
-             let pc' := add_word pc (if w == Z_to_word 0 then Z_to_word 1 
+             let pc' := add_word pc (if w == Z_to_word 0 then Z_to_word 1
                                      else imm_to_word n) in
              step (imem,dmem,reg,pc,true) (imem,dmem,reg,pc',true)
 | step_jal : forall imem dmem reg reg' pc i r w b,
              forall (FETCH : get imem pc = Some i),
              forall (INST : decode_instr i = Some (Jal _ r)),
              forall (RW : get reg r = Some w),
-             forall (GETCALL : get_syscall w = None),
              forall (UPD : upd reg ra (pc.+1) = Some reg'),
              forall (VALID : valid_jmp pc w = b),
              step (imem,dmem,reg,pc,true) (imem,dmem,reg',w,b)
-| step_syscall : forall imem dmem dmem' reg reg' pc i r w sc b,
-                 forall (FETCH : get imem pc = Some i),
-                 forall (INST : decode_instr i = Some (Jal _ r)),
-                 forall (RW : get reg r = Some w),
-                 forall (GETCALL : get_syscall w = Some sc),
-                 forall (CALL : sem sc (imem,dmem,reg,pc,true) = 
-                                Some (imem,dmem',reg',pc .+1,true)),
-                 forall (VALID : valid_jmp pc w = b), 
-                 step (imem,dmem,reg,pc,true) (imem,dmem',reg',pc .+1,b).
+| step_syscall : forall imem dmem dmem' reg reg' pc pc' sc,
+                 forall (FETCH : get imem pc = None),
+                 forall (GETCALL : get_syscall pc = Some sc),
+                 forall (CALL : sem sc (imem,dmem,reg,pc,true) =
+                                Some (imem,dmem',reg',pc',true)),
+                 step (imem,dmem,reg,pc,true) (imem,dmem',reg',pc',true).
 
 (*unused so far*)
 Hypothesis step_determ : forall s s' s'', step s s' -> step s s'' -> s' = s''.
@@ -142,28 +138,26 @@ Inductive step_a : state -> state -> Prop :=
              (FETCH: get imem pc = Some i)
              (MSAME: same_domain dmem dmem')
              (RSAME: same_domain reg reg'),
-             step_a (imem,dmem,reg,pc,true) (imem,dmem',reg',pc,true). 
+             step_a (imem,dmem,reg,pc,true) (imem,dmem',reg',pc,true).
 
 Definition succ (st : state) (st' : state) : bool :=
   let '(imem,_,reg,pc,_) := st in
   let '(_,_,_,pc',_) := st' in
   match (get imem pc) with
-    | Some i => 
+    | Some i =>
       (*XXX: Review this *)
       match decode_instr i with
         | Some (Jump r) => valid_jmp pc pc'
-        | Some (Jal r) => match get reg r with
-                            | Some w => match get_syscall w with
-                                          | Some sc => valid_jmp pc w
-                                          | None => valid_jmp pc pc'
-                                        end
-                            | None => false
-                          end
+        | Some (Jal r) => valid_jmp pc pc'
         | Some (Bnz r imm) => (pc' == pc .+1) || (pc' == pc + imm_to_word imm)
         | None => false
         | _ => pc' == pc .+1
       end
-    | None => false
+    | None =>
+      match get_syscall pc with
+        | Some sc => true (* Double-check *)
+        | None => false
+      end
   end.
 
 Definition initial (s : state) := True.
@@ -171,18 +165,18 @@ Definition initial (s : state) := True.
 Program Instance abstract_cfi_machine : cfi_machine t := {|
   state := state;
   initial s := initial s;
-  
+
   step := step;
   step_a := step_a;
 
   get_pc s := let '(_,_,_,pc,_) := s in pc;
-  
-  succ := succ      
+
+  succ := succ
  |}.
 Next Obligation.
 Admitted.
 Next Obligation.
-  inversion H; subst. reflexivity. 
+  inversion H; subst. reflexivity.
 Qed.
 
 Definition S (xs : list state) :=
@@ -214,10 +208,12 @@ Lemma step_succ_violation ast ast' :
    b = false.
 Proof.
   intros SUCC STEP.
-  inversion STEP; subst; simpl in SUCC; rewrite FETCH INST in SUCC;
-  try (rewrite eqxx in SUCC; congruence); 
-  try (destruct (w == 0)); try (rewrite eqxx ?orbT in SUCC); 
-  try (rewrite RW GETCALL in SUCC); auto.
+  inversion STEP; subst; simpl in SUCC; rewrite FETCH in SUCC;
+  try rewrite INST in SUCC;
+  try (rewrite eqxx in SUCC; congruence);
+  try (destruct (w == 0)); try (rewrite eqxx ?orbT in SUCC);
+  try (rewrite RW in SUCC);
+  try rewrite GETCALL in SUCC; auto.
 Qed.
 
 Lemma step_a_violation ast ast' :
@@ -226,19 +222,19 @@ Lemma step_a_violation ast ast' :
    b = true.
 Proof.
   intros STEP.
-  inversion STEP; subst. reflexivity. 
-Qed.  
+  inversion STEP; subst. reflexivity.
+Qed.
 
 Theorem cfi : cfi abstract_cfi_machine S.
 Proof.
-  unfold cfi. intros. 
+  unfold cfi. intros.
   apply interm_equiv_intermrev in INTERM.
   induction INTERM as [s s' STEP | s s' s'' xs STEP INTERM ].
-  + destruct (succ s s') eqn:SUCC.  
-    * (*case the step is in the control flow graph*) 
-      left. intros si sj IN2. 
+  + destruct (succ s s') eqn:SUCC.
+    * (*case the step is in the control flow graph*)
+      left. intros si sj IN2.
       destruct IN2 as [[? ?] | CONTRA]; [idtac | destruct CONTRA];
-      subst. auto. 
+      subst. auto.
     * (*case the step is outside the contro flow graph*)
       destruct STEP as [STEPA | STEP].
       - (*case it's an attacker step*)
@@ -249,7 +245,7 @@ Proof.
         inversion STEPA. subst. discriminate.
       - (*case it's a normal step*)
         right; exists s; exists s'; exists []; exists [].
-        simpl; repeat (split;auto). 
+        simpl; repeat (split;auto).
         intros ? ? IN2. destruct IN2.
         intros ? ? IN2. destruct IN2.
         unfold S. exists s'. split; auto.
@@ -267,7 +263,7 @@ Proof.
         { destruct IN2. }
         { clear IHxs.
           rewrite <- app_assoc in IN2.
-          simpl in IN2. 
+          simpl in IN2.
           destruct (in2_reverse IN2) as [IN2' | [EQ1 EQ2]].
           - apply TSAFE; assumption.
           - subst. apply interm_last_step in INTERM; subst.
@@ -280,14 +276,14 @@ Proof.
         induction xs using rev_ind.
         { destruct IN2. }
         { rewrite <- app_assoc in IN2.
-          simpl in IN2. 
-          destruct (in2_reverse IN2) as [IN2' | [EQ1 EQ2]]. 
+          simpl in IN2.
+          destruct (in2_reverse IN2) as [IN2' | [EQ1 EQ2]].
           - apply TSAFE; assumption.
           - subst. apply interm_last_step in INTERM; subst; auto.
             intro STEP. assert (CONTRA := step_succ_violation SUCC STEP).
             inversion STEPA; subst; discriminate. }
       - (*case it's a normal step*)
-        right. induction xs using rev_ind; [inversion INTERM | idtac]. 
+        right. induction xs using rev_ind; [inversion INTERM | idtac].
         apply interm_last_step in INTERM; subst.
         exists s'; exists s''; exists xs; exists [].
         simpl; rewrite <- app_assoc. repeat (split; auto).
@@ -311,11 +307,11 @@ Proof.
      apply interm_last_step in INTERM; subst.
      destruct VIO as [VSTEP SUCC].
      assert (FLAG := step_succ_violation SUCC VSTEP).
-     destruct s' as [[[[imem dmem] aregs] apc] b]; subst. 
+     destruct s' as [[[[imem dmem] aregs] apc] b]; subst.
      destruct STEP as [STEPA | STEP].
      - inversion STEPA.
      - inversion STEP. }
-Qed. 
+Qed.
 
 
 End WithClasses.
