sealing/symbolic.v
@@ -110,7 +110,11 @@ Definition mkkey (s : state t) : option (state t) :=
   if key <? max_key then 
     let key' := inc_key key in
     do! reg' <- upd reg syscall_ret (max_word@(KEY key));
-    Some (State mem reg' (pc + 1)%w@pct key')
+    do! ret  <- get reg ra;
+    match ret with
+    | _@DATA => Some (State mem reg' ret key')
+    | _ => None
+    end
   else
     None.
 
@@ -119,7 +123,11 @@ Definition seal (s : state t) : option (state t) :=
   match get reg syscall_arg1, get reg syscall_arg2 with
   | Some (payload@DATA), Some (_@(KEY key)) =>
     do! reg' <- upd reg syscall_ret (payload@(SEALED key));
-    Some (State mem reg' (pc + 1)%w@pct next_key)
+    do! ret  <- get reg ra;
+    match ret with
+    | _@DATA => Some (State mem reg' ret next_key)
+    | _ => None
+    end
   | _, _ => None
   end.
 
@@ -129,7 +137,11 @@ Definition unseal (s : state t) : option (state t) :=
   | Some (payload@(SEALED key)), Some (_@(KEY key')) =>
     if key == key' then
       do! reg' <- upd reg syscall_ret (payload@DATA);
-      Some (State mem reg' (pc + 1)%w@pct next_key)
+      do! ret  <- get reg ra;
+      match ret with
+      | _@DATA => Some (State mem reg' ret next_key)
+      | _ => None
+      end
     else None
   | _, _ => None
   end.
